Fix two examples

io/Compiler.Examples.fst
@@ -30,104 +30,102 @@ open Compiler.Model
 **)
 
 
-
-(** ** Test 1 - FO **)
+(** ** Testing **)
+(** *** Example 1 - FO **)
+let ex1_ct_pre = (fun () h -> True)
 let ex1_ct_post = (fun () h (rfd:resexn file_descr) lt -> (forall fd'. ~((EOpenfile "/etc/passwd" fd') `List.memP` lt)) /\ (Inl? rfd ==> is_open (Inl?.v rfd) (rev lt @ h)))
 let ex1_spec_pi : monitorable_prop = (fun cmd arg h -> match cmd, arg with | Openfile, s -> if s = "/etc/passwd" then false else true | _ -> true)
 let ex1_inst_pi : monitorable_prop = ex1_spec_pi
 let ex1_ct_rc = (fun () h (rfd:resexn file_descr) lt -> Inl? rfd && (is_open (Inl?.v rfd) (rev lt @ h)))
 
-let rec ex1_c1post0 (h:trace) (lt:trace) : Lemma
-  (requires (enforced_locally ex1_spec_pi h lt))
-  (ensures (ex1_ct_post () h (Inr Contract_failure) lt))
-  (decreases lt) =
-  match lt with
-  | [] -> ()
-  | e :: tail -> ex1_c1post0 (e::h) tail
+val ex1_c1post : squash (forall h lt. ex1_ct_pre () h /\ enforced_locally ex1_spec_pi h lt ==> (ex1_ct_post () h (Inr Contract_failure) lt))
+let ex1_c1post = 
+  let rec aux (h:trace) (lt:trace) : Lemma
+    (requires (enforced_locally ex1_spec_pi h lt))
+    (ensures (ex1_ct_post () h (Inr Contract_failure) lt))
+    (decreases lt) = (
+    match lt with
+    | [] -> ()
+    | e :: tail -> aux (e::h) tail) in
+  Classical.forall_intro_2 (Classical.move_requires_2 aux)
 
-val ex1_c1post : squash (forall h lt. enforced_locally ex1_spec_pi h lt ==> (ex1_ct_post () h (Inr Contract_failure) lt))
-let ex1_c1post = Classical.forall_intro_2 (Classical.move_requires_2 ex1_c1post0)
-
-val ex1_c2post : squash (forall x h r lt. enforced_locally ex1_spec_pi h lt /\ (ex1_ct_rc x h r lt) ==> ex1_ct_post x h r lt)
+val ex1_c2post : squash (forall x h r lt. ex1_ct_pre () h /\ enforced_locally ex1_spec_pi h lt /\ (ex1_ct_rc x h r lt) ==> ex1_ct_post x h r lt)
 let ex1_c2post = ()
-
-let rec ex1_stronger_pis0 (h:trace) (lt:trace) : Lemma
-  (requires (enforced_locally ex1_inst_pi h lt))
-  (ensures (enforced_locally ex1_spec_pi h lt))
-  (decreases lt) =
-  match lt with
-  | [] -> ()
-  | e :: tail -> ex1_stronger_pis0 (e::h) tail
                                                   
 val ex1_stronger_pis : squash (forall h lt. enforced_locally ex1_inst_pi h lt ==> enforced_locally ex1_spec_pi h lt)
-let ex1_stronger_pis = Classical.forall_intro_2 (Classical.move_requires_2 ex1_stronger_pis0)
+let ex1_stronger_pis = 
+  let rec aux (h:trace) (lt:trace) : Lemma
+    (requires (enforced_locally ex1_inst_pi h lt))
+    (ensures (enforced_locally ex1_spec_pi h lt))
+    (decreases lt) = (match lt with
+    | [] -> ()
+    | e :: tail -> aux (e::h) tail) in 
+  Classical.forall_intro_2 (Classical.move_requires_2 aux)
 
-let ex1_interface : src_interface = {
-  spec_pi = ex1_spec_pi;
-  inst_pi = ex1_inst_pi;
+let ex1 : src_interface = {
+  spec_pi = ex1_spec_pi; inst_pi = ex1_inst_pi;
+  inst_pi_stronger_spec_pi = ex1_stronger_pis;
 
-  pt = (fun fl -> (unit -> IIO (resexn unit) (fl + IOActions) (fun _ -> True) (fun _ _ _ -> True)));
-
-  ct = (fun fl -> unit -> IIO (resexn file_descr) fl (fun _ -> True) (ex1_ct_post ()));
+  ct = (fun fl -> unit -> IIO (resexn file_descr) fl (ex1_ct_pre ()) (ex1_ct_post ()));
   ct_rcs = Node (| unit, resexn file_descr, ex1_ct_rc |) Leaf Leaf;
-
 
   ct_importable = (fun fl -> 
     safe_importable_arrow_pre_post_args unit _ _ _ ex1_c1post ex1_c2post);
-  
-  inst_pi_stronger_spec_pi = ex1_stronger_pis;
+  p_post = (fun _ _ _ lt -> (forall fd'. ~((EOpenfile "/etc/passwd" fd') `List.memP` lt)));
 }
 
-val ex1_prog : prog_src ex1_interface
-let ex1_prog #fl ctx () : IIO (resexn unit) (fl + IOActions) (fun _ -> True) (fun _ _ _ -> True) =
+val ex1_prog : prog_src ex1
+let ex1_prog #fl ctx args : IIO int (fl + IOActions) (fun _ -> True) (ex1.p_post args) =
+  //let test = static_cmd Openfile "/etc/passwd" in
   let _ = ctx () in
-  Inl ()
+  0 
 
-val ex1_ctx : ctx_src ex1_interface
+val ex1_ctx : ctx_src ex1
 let ex1_ctx #fl io_acts eff_rcs () : IIO (resexn file_descr) fl (fun _ -> True) (ex1_ct_post ()) = 
   io_acts Openfile "/etc/passwd"
 
-val ex1_ctx_t : ctx_tgt (comp_int_src_tgt ex1_interface)
-let ex1_ctx_t #fl io_acts () : IIOpi (resexn file_descr) fl (comp_int_src_tgt ex1_interface).spec_pi = 
+val ex1_ctx_t : ctx_tgt (comp_int_src_tgt ex1)
+let ex1_ctx_t #fl io_acts () : IIOpi (resexn file_descr) fl (comp_int_src_tgt ex1).spec_pi = 
   io_acts Openfile "/etc/passwd"
 
-(** ** Test 3 - HO 1 **)
+(** ** Example 2 - HO left 1 **)
 
 let ex3_pi : monitorable_prop = (fun _ _ _ -> true)
-assume val ex3_stronger_pis : squash (forall h lt. enforced_locally ex3_pi h lt ==> enforced_locally ex3_pi h lt)
+let ex3_post = (fun h (rfd:resexn file_descr) lt -> Inl? rfd ==> is_open (Inl?.v rfd) (rev lt @ h))
 
+assume val ex3_stronger_pis : squash (forall h lt. enforced_locally ex3_pi h lt ==> enforced_locally ex3_pi h lt)
 
 let ex3_rcs : tree pck_rc =  
   Node (| unit, resexn file_descr, (fun () h (rfd:resexn file_descr) lt -> Inl? rfd && (is_open (Inl?.v rfd) (rev lt @ h))) |) 
-              (Node (| file_descr, unit, (fun fd h _ _ -> is_open fd h) |) Leaf Leaf)
-              Leaf
+     (Node (| file_descr, unit, (fun fd h _ _ -> is_open fd h) |) Leaf Leaf)
+     Leaf
+  
+assume val ex3_c1post : squash (forall h lt. enforced_locally ex3_pi h lt ==> (exists (rfd:resexn file_descr). Inl? rfd ==> is_open (Inl?.v rfd) (rev lt @ h)))
+val ex3_c2post : squash (forall h (rfd:resexn file_descr) lt. Inl? rfd && (is_open (Inl?.v rfd) (rev lt @ h)) ==> (Inl? rfd ==> is_open (Inl?.v rfd) (rev lt @ h)))
+let ex3_c2post = ()
 
-let test_ho_interface : src_interface = {
+let ex3 : src_interface = {
   spec_pi = ex3_pi;
   inst_pi = ex3_pi;
   inst_pi_stronger_spec_pi = ex3_stronger_pis;
 
-  pt = (fun fl -> (unit -> IIO (resexn unit) (fl + IOActions) (fun _ -> True) (fun _ _ _ -> true)));
-
-  ct = (fun fl -> (fd:file_descr -> IIO (resexn unit) fl (fun h -> is_open fd h) (fun _ _ lt -> lt == [])) -> IIO (resexn file_descr) fl (fun _ -> True) (fun h rfd lt -> Inl? rfd ==> is_open (Inl?.v rfd) (rev lt @ h)));
+  ct = (fun fl -> (fd:file_descr -> IIO (resexn unit) fl (fun h -> is_open fd h) (fun _ _ lt -> lt == [])) -> IIO (resexn file_descr) fl (fun _ -> True) ex3_post);
   ct_rcs = ex3_rcs;
 
   ct_importable = (fun fl -> 
-    let exportable_cb = exportable_arrow_pre_post_args file_descr unit #ex3_pi #(left ex3_rcs) #fl (fun fd h -> is_open fd h) (fun fd _ _ lt -> lt == []) #() #() in
-    let c1post : unit -> squash (forall h lt. enforced_locally (fun _ _ _ -> true) h lt ==> (exists (rfd:resexn file_descr). Inl? rfd ==> is_open (Inl?.v rfd) (rev lt @ h))) = (fun () ->
-      admit ()) in
-    let c2post : squash (forall h (rfd:resexn file_descr) lt. Inl? rfd && (is_open (Inl?.v rfd) (rev lt @ h)) ==> (Inl? rfd ==> is_open (Inl?.v rfd) (rev lt @ h))) = () in
-    safe_importable_arrow_pre_post exportable_cb importable_file_descr (fun _ -> True) (fun h rfd lt -> Inl? rfd ==> is_open (Inl?.v rfd) (rev lt @ h)) (c1post ()) ());
+    let exportable_cb = exportable_arrow_pre_post_args file_descr unit #ex3_pi #(left ex3_rcs) #fl (fun fd h -> is_open fd h) (fun fd _ _ lt -> lt == []) in
+    safe_importable_arrow_pre_post exportable_cb importable_file_descr (fun _ -> True) (fun h rfd lt -> Inl? rfd ==> is_open (Inl?.v rfd) (rev lt @ h)) ex3_c1post ex3_c2post);
+
+  p_post = (fun _ _ _ _ -> True);
 }
 
-
-val test_ho_prog : prog_src test_ho_interface
-let test_ho_prog #fl ctx () : IIO (resexn unit) (fl + IOActions) (fun _ -> True) (fun _ _ _ -> True) =
+val ex3_prog : prog_src ex3
+let ex3_prog #fl ctx args =
   let _ = ctx (fun fd -> Inl ()) in
-  Inl ()
+  0
 
-val test_ho_ctx : ctx_src test_ho_interface
-let test_ho_ctx #fl io_acts eff_rcs cb : IIO (resexn file_descr) fl (fun _ -> True) (fun h rfd lt -> Inl? rfd ==> is_open (Inl?.v rfd) (rev lt @ h)) = 
+val ex3_ctx : ctx_src ex3 
+let ex3_ctx #fl io_acts eff_rcs cb : IIO (resexn file_descr) fl (fun _ -> True) (fun h rfd lt -> Inl? rfd ==> is_open (Inl?.v rfd) (rev lt @ h)) = 
   let post1 = root eff_rcs in
   let (| _, pre1 |) = root (left eff_rcs) in 
   let rfd = io_acts Openfile "/etc/passwd" in
@@ -135,8 +133,13 @@ let test_ho_ctx #fl io_acts eff_rcs cb : IIO (resexn file_descr) fl (fun _ -> Tr
   | Inl fd -> let _ = pre1 fd in rfd
   | _ -> rfd
 
-(** can't type this without defining ct_importable
-val test_ho_ctx_t : ctx_ilang (comp_int_iio_ilang test_ho_interface)
-let test_ho_ctx_t #fl io_acts cb : IIOpi (resexn file_descr) fl (comp_int_iio_ilang test_ho_interface).spec_pi = 
-  io_acts Openfile "/etc/passwd"
-**)
+val ex3_ctx_t : ctx_tgt (comp_int_src_tgt ex3)
+let ex3_ctx_t #fl io_acts cb : IIOpi (resexn file_descr) fl (comp_int_src_tgt ex3).spec_pi = 
+  let rfd = io_acts Openfile "/etc/passwd" in
+  match rfd with
+  | Inl fd -> begin
+    //let _ = io_acts Close fd in 
+    let _ = cb fd in 
+    rfd
+  end
+  | _ -> rfd
